Reducing the number of theorems we need to prove by removing the specific definitions for when the encoding process starts from the specific state 0, and instead proving things only using the more generic definitions which allow you to start from any state.

ConvolutionalCodes/state_machineScript.sml
@@ -125,47 +125,27 @@ Theorem wfmachine_transition_fn_output_length[simp] = cj 5 (iffLR wfmachine_def)
 Theorem wfmachine_output_length_greater_than_zero[simp] = cj 6 (iffLR wfmachine_def);
 
 (* -------------------------------------------------------------------------- *)
-(* Helper function that does the actual work to encode a binary string using  *)
-(* convolutional coding, according to a chosen state machine.                 *)
-(*                                                                            *)
-(* This function additionally has a parameter to keep track of the current    *)
-(* state that the state machine is in.                                        *)
+(* Encodes a binary string using convolutional coding, according to a chosen  *)
+(* state machine, starting from a given state                                 *)
 (* -------------------------------------------------------------------------- *)
-Definition vd_encode_from_state_def:
-  vd_encode_from_state _ [] _ = [] ∧
-  vd_encode_from_state (m : state_machine) (b::bs : bool list) (s : num) =
+Definition vd_encode_def:
+  vd_encode _ [] _ = [] ∧
+  vd_encode (m : state_machine) (b::bs : bool list) (s : num) =
   let
     d = m.transition_fn <| origin := s; input := b; |>
   in
-    d.output ⧺ vd_encode_from_state m bs d.destination
+    d.output ⧺ vd_encode m bs d.destination
 End
-
-(* -------------------------------------------------------------------------- *)
-(* Encodes a binary string using convolutional coding, according to a chosen  *)
-(* state machine                                                              *)
-(* -------------------------------------------------------------------------- *)
-Definition vd_encode_def:
-  vd_encode (m : state_machine) bs = vd_encode_from_state m bs 0
-End
-
-(* -------------------------------------------------------------------------- *)
-(* Helper function to calculate the final state you'll end up in if you apply *)
-(* the given state machine to the given bitstring. Also has a variable to     *)
-(* keep track of the current state we're in.                                  *)
-(* -------------------------------------------------------------------------- *)
-Definition vd_encode_state_from_state_def:
-  vd_encode_state_from_state (m : state_machine) [] s = s ∧
-  vd_encode_state_from_state m (b::bs) s =
-  vd_encode_state_from_state m bs (m.transition_fn <| origin := s; input := b; |>).destination
-End 
 
 (* -------------------------------------------------------------------------- *)
 (* Calculates the final state you'll end up in if you apply the given state   *)
-(* machine to the given bitstring.                                            *)
+(* machine to the given bitstring, given an initial state                     *)
 (* -------------------------------------------------------------------------- *)
 Definition vd_encode_state_def:
-  vd_encode_state (m : state_machine) bs = vd_encode_state_from_state m bs 0
-End
+  vd_encode_state (m : state_machine) [] s = s ∧
+  vd_encode_state m (b::bs) s =
+  vd_encode_state m bs (m.transition_fn <| origin := s; input := b; |>).destination
+End 
 
 Definition all_transitions_helper_def:
   all_transitions_helper (m : state_machine) (b : bool) = GENLIST (λn. <| origin := n; input := b |>) m.num_states
@@ -202,14 +182,14 @@ End
 
 (* -------------------------------------------------------------------------- *)
 (* Returns true if it is possible to reach the state s at time t when         *)
-(* starting at 0.                                                             *)
+(* starting at the initial state i                                            *)
 (* -------------------------------------------------------------------------- *)
 Definition is_reachable_def:
-  is_reachable m s t = ∃bs. (LENGTH bs = t ∧ vd_encode_state m bs = s)
+  is_reachable m i s t = ∃bs. (LENGTH bs = t ∧ vd_encode_state m bs i = s)
 End
 
 Theorem vd_encode_empty[simp]:
-  ∀m. vd_encode m [] = []
+  ∀m s. vd_encode m [] s = []
 Proof
   rpt strip_tac
   >> EVAL_TAC
@@ -218,91 +198,42 @@ QED
 (* -------------------------------------------------------------------------- *)
 (* See comment for vd_encode_cons                             *)
 (* -------------------------------------------------------------------------- *)
-Theorem vd_encode_from_state_cons:
-  ∀m b bs s.
-    vd_encode_from_state m (b :: bs) s =
-    (m.transition_fn <| origin := s; input := b; |>).output ⧺ (vd_encode_from_state m bs (m.transition_fn <| origin := s; input := b; |>).destination)
-Proof
-  rpt strip_tac
-  >> gvs[vd_encode_from_state_def]
-  >> gvs[vd_encode_state_from_state_def]
-QED
-
-(* -------------------------------------------------------------------------- *)
-(* Can break convolutional encoding up into doing a step, with the rest of    *)
-(* the encoding appended on, starting from the appropriate state              *)
-(* -------------------------------------------------------------------------- *)
 Theorem vd_encode_cons:
-  ∀m b bs. vd_encode m (b :: bs) =
-           (m.transition_fn <| origin := 0; input := b; |>).output ⧺ (vd_encode_from_state m bs (m.transition_fn <| origin := 0; input := b; |>).destination)
+  ∀m b bs s.
+    vd_encode m (b :: bs) s =
+    (m.transition_fn <| origin := s; input := b; |>).output ⧺ (vd_encode m bs (m.transition_fn <| origin := s; input := b; |>).destination)
 Proof
   rpt strip_tac
   >> gvs[vd_encode_def]
   >> gvs[vd_encode_state_def]
-  >> PURE_ONCE_REWRITE_TAC[vd_encode_from_state_cons]
-  >> gvs[]
 QED
 
 (* -------------------------------------------------------------------------- *)
 (* See comment for vd_encode_append                           *)
 (* -------------------------------------------------------------------------- *)
-Theorem vd_encode_from_state_append:
+Theorem vd_encode_append:
   ∀m bs cs s.
-    vd_encode_from_state m (bs ⧺ cs) s =
-    vd_encode_from_state m bs s ⧺ vd_encode_from_state m cs (vd_encode_state_from_state m bs s)          
+    vd_encode m (bs ⧺ cs) s =
+    vd_encode m bs s ⧺ vd_encode m cs (vd_encode_state m bs s)          
 Proof
   gen_tac
   >> Induct_on ‘bs’
   >- (rpt strip_tac >> EVAL_TAC)
   >> rpt strip_tac
   >> gvs[APPEND]
-  >> gvs[vd_encode_from_state_cons]
-  >> gvs[vd_encode_state_from_state_def]
+  >> gvs[vd_encode_cons]
+  >> gvs[vd_encode_state_def]
 QED
 
-(* -------------------------------------------------------------------------- *)
-(* Can break convolutional encoding up into two halves: doing a bunch of      *)
-(* steps from the initial state, then doing a bunch of steps from the state   *)
-(* that is reached at this point.                                             *)
-(* -------------------------------------------------------------------------- *)
-Theorem vd_encode_append:
-  ∀m bs cs.
-    vd_encode m (bs ⧺ cs) =
-    (vd_encode m bs) ⧺ (vd_encode_from_state m cs (vd_encode_state m bs))
-Proof
-  rpt strip_tac
-  >> gvs[vd_encode_def, vd_encode_state_def]
-  >> gvs[vd_encode_from_state_append]
-QED
-
-(* -------------------------------------------------------------------------- *)
-(* Can break convolutional encoding up into doing a bunch of steps from the   *)
-(* initial state, then doing a final step from the final state.               *)
-(* -------------------------------------------------------------------------- *)
-Theorem vd_encode_snoc:
-  ∀m b bs. vd_encode m (SNOC b bs) =
-           (vd_encode m bs) ⧺ (vd_encode_from_state m [b] (vd_encode_state m bs))
-Proof
-  gvs[SNOC]
-  >> gvs[vd_encode_append]
-QED
-
-Theorem vd_encode_state_from_state_snoc:
+Theorem vd_encode_state_snoc:
   ∀m b bs s.
-    vd_encode_state_from_state m (SNOC b bs) s = (m.transition_fn <| origin := (vd_encode_state_from_state m bs s); input := b; |>).destination
+    vd_encode_state m (SNOC b bs) s = (m.transition_fn <| origin := (vd_encode_state m bs s); input := b; |>).destination
 Proof
   Induct_on ‘bs’
   >- (rpt strip_tac >> EVAL_TAC)
   >> rpt strip_tac
   >> gvs[]
-  >> gvs[vd_encode_state_from_state_def]
-QED
-
-Theorem vd_encode_state_snoc:
-  ∀m b bs.
-    vd_encode_state m (SNOC b bs) = (m.transition_fn <| origin := (vd_encode_state m bs); input := b; |>).destination
-Proof
-  gvs[vd_encode_state_def, vd_encode_state_from_state_snoc]
+  >> gvs[vd_encode_state_def]
 QED
 
 Theorem all_transitions_helper_mem_is_valid[simp]:
@@ -472,29 +403,18 @@ Proof
   >> gvs[CONS]
 QED
 
-Theorem vd_encode_from_state_length[simp]:
+Theorem vd_encode_length[simp]:
   ∀m bs s.
     wfmachine m ∧
     s < m.num_states ⇒
-    LENGTH (vd_encode_from_state m bs s) = m.output_length * LENGTH bs
+    LENGTH (vd_encode m bs s) = m.output_length * LENGTH bs
 Proof
   gen_tac
   >> Induct_on ‘bs’
   >- (rpt strip_tac >> EVAL_TAC)
   >> rpt strip_tac
-  >> gvs[vd_encode_from_state_cons]
+  >> gvs[vd_encode_cons]
   >> gvs[ADD1]
-QED
-
-Theorem vd_encode_length[simp]:
-  ∀m bs.
-    wfmachine m ⇒
-    LENGTH (vd_encode m bs) = m.output_length * LENGTH bs
-Proof
-  rpt strip_tac
-  >> gvs[vd_encode_def]
-  >> DEP_PURE_ONCE_REWRITE_TAC [vd_encode_from_state_length]
-  >> gvs[]
 QED
 
 Theorem transition_fn_destination_is_valid[simp]:
@@ -507,29 +427,19 @@ Proof
   >> gvs[]
 QED
 
-Theorem vd_encode_state_from_state_is_valid[simp]:
+Theorem vd_encode_state_is_valid[simp]:
   ∀m bs s.
     wfmachine m ∧ 
     s < m.num_states ⇒
-    vd_encode_state_from_state m bs s < m.num_states
+    vd_encode_state m bs s < m.num_states
 Proof
   gen_tac
   >> Induct_on ‘bs’
   >- (rpt strip_tac
-      >> gvs[vd_encode_state_from_state_def]
+      >> gvs[vd_encode_state_def]
      )
   >> rpt strip_tac
-  >> gvs[vd_encode_state_from_state_def]
-QED
-
-Theorem vd_encode_state_is_valid[simp]:
-  ∀m bs.
-    wfmachine m ⇒
-    vd_encode_state m bs < m.num_states
-Proof
-  rpt strip_tac
   >> gvs[vd_encode_state_def]
-  >> DEP_PURE_ONCE_REWRITE_TAC[vd_encode_state_from_state_is_valid]
 QED
 
 Theorem transition_fn_output_length_0[simp]:
@@ -544,29 +454,17 @@ Proof
   >> metis_tac[wfmachine_transition_fn_output_length]
 QED
 
-Theorem vd_encode_from_state_output_length_0[simp]:
+Theorem vd_encode_output_length_0[simp]:
   ∀m bs s.
     wfmachine m ∧
     s < m.num_states ∧
     m.output_length = 0 ⇒
-    vd_encode_from_state m bs s = []
+    vd_encode m bs s = []
 Proof
   gen_tac
   >> Induct_on ‘bs’ >> rpt strip_tac
-  >- gvs[vd_encode_from_state_def]
-  >> gvs[vd_encode_from_state_cons]
-QED
-
-Theorem vd_encode_output_length_0[simp]:
-  ∀m bs s.
-    wfmachine m ∧
-    m.output_length = 0 ⇒
-    vd_encode m bs = []
-Proof
-  gvs[vd_encode_def]
-  >> rpt strip_tac
-  >> irule vd_encode_from_state_output_length_0
-  >> gvs[]
+  >- gvs[vd_encode_def]
+  >> gvs[vd_encode_cons]
 QED
 
 Theorem all_transitions_helper_valid:
@@ -617,9 +515,8 @@ Proof
   >> gvs[transition_component_equality_local]
 QED
 
-Theorem is_reachable_zero_zero[simp]:
-  ∀m.
-    is_reachable m 0 0
+Theorem is_reachable_init_zero[simp]:
+  ∀m i. is_reachable m i i 0
 Proof
   rpt strip_tac
   >> EVAL_TAC
@@ -627,10 +524,10 @@ Proof
   >> EVAL_TAC
 QED
 
-Theorem not_is_reachable_nonzero_zero[simp]:
-  ∀m s.
-    s ≠ 0 ⇒
-    ¬is_reachable m s 0
+Theorem not_is_reachable_noninit_zero[simp]:
+  ∀m i s.
+    s ≠ i ⇒
+    ¬is_reachable m i s 0
 Proof
   rpt gen_tac
   >> disch_tac
@@ -642,8 +539,8 @@ Proof
 QED
 
 Theorem is_reachable_transition_fn:
-  ∀m s t b.
-    is_reachable m s t ⇒ is_reachable m (m.transition_fn <| origin := s; input := b |>).destination (SUC t)
+  ∀m i s t b.
+    is_reachable m i s t ⇒ is_reachable m i (m.transition_fn <| origin := s; input := b |>).destination (SUC t)
 Proof
   rpt strip_tac
   >> gvs[is_reachable_def]
@@ -653,30 +550,31 @@ Proof
 QED
 
 Theorem is_reachable_transition_fn_destination:
-  ∀m r t.
-    is_reachable m r.origin t ⇒ is_reachable m (m.transition_fn r).destination (SUC t)
+  ∀m i r t.
+    is_reachable m i r.origin t ⇒ is_reachable m i (m.transition_fn r).destination (SUC t)
 Proof
   rpt strip_tac
-  >> qspecl_then [‘m’, ‘r.origin’, ‘t’, ‘r.input’] assume_tac is_reachable_transition_fn
+  >> qspecl_then [‘m’, ‘i’, ‘r.origin’, ‘t’, ‘r.input’] assume_tac is_reachable_transition_fn
   >> gvs[]
 QED
 
 Theorem is_reachable_suc:
-  ∀m s t.
-    is_reachable m s (SUC t) ⇔ ∃s' b. is_reachable m s' t ∧ (m.transition_fn <| origin := s'; input := b |>).destination = s
+  ∀m i s t.
+    is_reachable m i s (SUC t) ⇔ ∃s' b. is_reachable m i s' t ∧ (m.transition_fn <| origin := s'; input := b |>).destination = s
 Proof
   rpt strip_tac
   >> EQ_TAC
   >- (disch_tac
       >> gvs[is_reachable_def]
-      >> qexistsl [‘vd_encode_state m (FRONT bs)’, ‘LAST bs’]
+      >> qexistsl [‘vd_encode_state m (FRONT bs) i’, ‘LAST bs’]
       >> conj_tac
       >- (qexists ‘FRONT bs’
           >> gvs[]
           >> Cases_on ‘bs’ using SNOC_CASES >> gvs[])
       >> Cases_on ‘bs’ using SNOC_CASES
       >- gvs[]
-      >> gvs[vd_encode_state_snoc])
+      >> gvs[vd_encode_state_snoc]
+     )
   >> rpt strip_tac
   >> gvs[]
   >> irule is_reachable_transition_fn
@@ -684,8 +582,8 @@ Proof
 QED
 
 Theorem is_reachable_suc_transition_fn_destination:
-  ∀m s t.
-    is_reachable m s (SUC t) ⇔ ∃r. is_reachable m r.origin t ∧ (m.transition_fn  r).destination = s
+  ∀m i s t.
+    is_reachable m i s (SUC t) ⇔ ∃r. is_reachable m i r.origin t ∧ (m.transition_fn  r).destination = s
 Proof
   rpt strip_tac
   >> gvs[]
@@ -699,36 +597,28 @@ Proof
   >> gvs[]
 QED
 
-Theorem vd_encode_state_from_state_empty[simp]:
-  ∀m s.
-    vd_encode_state_from_state m [] s = s
-Proof
-  rpt strip_tac
-  >> gvs[vd_encode_state_from_state_def]
-QED
-
 Theorem vd_encode_state_empty[simp]:
-  ∀m.
-    vd_encode_state m [] = 0
+  ∀m s.
+    vd_encode_state m [] s = s
 Proof
   rpt strip_tac
   >> gvs[vd_encode_state_def]
 QED
 
-Theorem is_reachable_zero[simp]:
-  ∀m s.
-    is_reachable m s 0 ⇔ s = 0
+Theorem is_reachable_init[simp]:
+  ∀m i s.
+    is_reachable m i s 0 ⇔ s = i
 Proof
   rpt strip_tac
   >> gvs[is_reachable_def]
 QED
 
-Theorem vd_encode_from_state_singleton[simp]:
+Theorem vd_encode_singleton[simp]:
   ∀m b s.
-    vd_encode_from_state m [b] s = (m.transition_fn <| origin := s; input := b |>).output
+    vd_encode m [b] s = (m.transition_fn <| origin := s; input := b |>).output
 Proof
   rpt strip_tac
-  >> gvs[vd_encode_from_state_def]
+  >> gvs[vd_encode_def]
 QED
 
 (* -------------------------------------------------------------------------- *)
@@ -829,7 +719,7 @@ End
 (* I would expect if I manually did the computation myself                    *)
 (* -------------------------------------------------------------------------- *)
 Theorem vd_encode_test1:
-  vd_encode example_state_machine [F; T; T; T; F] = [F; F; T; T; F; F; T; F; F; T]  
+  vd_encode example_state_machine [F; T; T; T; F] 0 = [F; F; T; T; F; F; T; F; F; T]  
 Proof
   EVAL_TAC
 QED
